changing prf_mac lemmas to account for new flags scheme ***NO_CI***

examples/low-level/crypto/Crypto.AEAD.PRF_MAC.fst
@@ -1,5 +1,4 @@
 module Crypto.AEAD.PRF_MAC
-
 open FStar.UInt32
 open FStar.HyperStack
 open FStar.Monotonic.RRef
@@ -81,7 +80,7 @@ let prf_mac_wrapper i t k_0 x =
  *)
 
 let unused_mac_exists (#i:id) (t:PRF.state i) (x:PRF.domain_mac i) (h:HS.mem) =
-  safeId i ==>
+  prf i ==>
     (let table = HS.sel h (PRF.itable i t) in
      match PRF.find_mac table x with
      | None     -> False                                            //the mac entry definitely exsits in the PRF log
@@ -121,13 +120,13 @@ private val none_above_otp_after_prf_mac
   (mac:CMA.state (i,x.iv))
   (h0 h1:mem) : Lemma
   (requires inv aead_st h0 /\
-            (safeId i ==> fresh_nonce x.iv aead_st h0) /\
+            (safeMac i ==> fresh_nonce_st x.iv aead_st h0) /\
             prf_mac_ensures i aead_st.prf k_0 x h0 mac h1)
-  (ensures  (safeId i ==>
+  (ensures  (safeMac i ==>
               (let prf_table_1 = HS.sel h1 (PRF.itable i aead_st.prf) in
                none_above (PRF.incr i x) prf_table_1)))
 let none_above_otp_after_prf_mac #i #rw aead_st k_0 x mac h0 h1 =
-  if safeId i then begin
+  if safeMac i then begin
     let prf_table_0 = HS.sel h0 (itable i aead_st.prf) in 
     (match find_mac prf_table_0 x with
      | Some _ -> ()
@@ -143,84 +142,97 @@ val unused_mac_exists_after_prf_mac
   (mac:CMA.state (i,x.iv))
   (h0 h1:mem) : Lemma
   (requires inv aead_st h0 /\
-            (safeId i ==> fresh_nonce x.iv aead_st h0) /\
+            (safeMac i ==> fresh_nonce_st x.iv aead_st h0) /\
             prf_mac_ensures i aead_st.prf k_0 x h0 mac h1)
-  (ensures (safeId i ==> unused_mac_exists aead_st.prf x h1))
+  (ensures (safeMac i ==> unused_mac_exists aead_st.prf x h1))
 let unused_mac_exists_after_prf_mac #i #rw aead_st k_0 x mac h0 h1 = ()
 
-val frame_prf_find_snoc_iv
-  (#r:region)
+val inv_after_prf_mac
   (#i:id)
-  (prf_table:prf_table r i)
-  (entry:entry r i)
-  (x:domain i) : Lemma
-  (requires (x.iv <> entry.x.iv))
-  (ensures (PRF.find prf_table x == PRF.find (SeqProperties.snoc prf_table entry) x))
-let frame_prf_find_snoc_iv #r #i prf_table entry x = SeqProperties.find_snoc prf_table entry (is_entry_domain x)
+  (#rw:rw)
+  (aead_st:aead_state i rw)
+  (k_0:CMA.akey aead_st.prf.mac_rgn i)
+  (x:PRF.domain_mac i)
+  (mac:CMA.state (i,x.iv))
+  (h0 h1:mem) : Lemma
+  (requires inv aead_st h0 /\                                  //invariant holds in h0
+            (safeMac i ==> fresh_nonce_st x.iv aead_st h0) /\  //the nonce is fresh w.r.t. the AEAD table
+            prf_mac_ensures i aead_st.prf k_0 x h0 mac h1)     //prf_mac_ensures holds from h0 to h1
+  (ensures //TODO: inv aead_st h1 /\                                  //invariant holds in h1
+           (safeMac i ==>
+             (let prf_table = HS.sel h1 (itable i aead_st.prf) in
+	      unused_mac_exists aead_st.prf x h1 /\        //unused mac exists in the prf table
+              none_above (PRF.incr i x) prf_table)))      //no otp entries exist in the prf table for this nonce
+let inv_after_prf_mac #i #rw aead_st k_0 x mac h0 h1 =
+  if safeMac i
+  then begin
+    unused_mac_exists_after_prf_mac aead_st k_0 x mac h0 h1;  //establish unused_mac_exists
+    none_above_otp_after_prf_mac aead_st k_0 x mac h0 h1      //establish none_above
+  end
 
-open Crypto.AEAD.Encoding
-open Crypto.Plain
-open Crypto.Symmetric.Bytes
+(* open Crypto.AEAD.Encoding *)
+(* open Crypto.Plain *)
+(* open Crypto.Symmetric.Bytes *)
 
-let frame_mac_is_set_snoc_iv
-  (#r:region)
-  (#i:id)
-  (prf_table:prf_table r i{safeId i})
-  (iv:Crypto.Symmetric.Cipher.iv (alg i))
-  (ad:adata)
-  (l:plainLen)
-  (cipher:lbytes l)
-  (tag:MAC.tag)
-  (h:mem)
-  (entry:entry r i) : Lemma
-  (requires (mac_is_set prf_table iv ad l cipher tag h /\
-             iv <> entry.x.iv))
-  (ensures  (mac_is_set (SeqProperties.snoc prf_table entry) iv ad l cipher tag h))
-  = let dom_0 = {iv = iv; ctr = PRF.ctr_0 i} in
-    SeqProperties.find_snoc prf_table entry (is_entry_domain dom_0)
+(* let frame_mac_is_set_snoc_iv *)
+(*   (#r:region) *)
+(*   (#i:id) *)
+(*   (prf_table:prf_table r i{safeId i}) *)
+(*   (iv:Crypto.Symmetric.Cipher.iv (alg i)) *)
+(*   (ad:adata) *)
+(*   (l:plainLen) *)
+(*   (cipher:lbytes l) *)
+(*   (tag:MAC.tag) *)
+(*   (h:mem) *)
+(*   (entry:entry r i) : Lemma *)
+(*   (requires (mac_is_set prf_table iv ad l cipher tag h /\ *)
+(*              iv <> entry.x.iv)) *)
+(*   (ensures  (mac_is_set (SeqProperties.snoc prf_table entry) iv ad l cipher tag h)) *)
+(*   = let dom_0 = {iv = iv; ctr = PRF.ctr_0 i} in *)
+(*     SeqProperties.find_snoc prf_table entry (is_entry_domain dom_0) *)
 
-let rec lemma_counterblocks_iv
-  (i:id{safeId i})
-  (r:eternal_region)
-  (x:PRF.domain i{PRF.ctr_0 i <^ PRF.(x.ctr)})
-  (l:nat)
-  (from_pos:nat)
-  (to_pos:nat{from_pos <= to_pos /\ to_pos <= l /\ safelen i (to_pos - from_pos) PRF.(x.ctr)})
-  (plain:Crypto.Plain.plain i l)
-  (cipher:lbytes l) : Lemma
-  (requires True)
-  (ensures (let otp_entries = counterblocks i r x l from_pos to_pos plain cipher in
-            forall (prf_entry:entry r i).
-              otp_entries `SeqProperties.contains` prf_entry ==> prf_entry.x.iv = x.iv))
-  (decreases (to_pos - from_pos))
-  = let blockl = v (Crypto.Symmetric.Cipher.(blocklen (cipherAlg_of_id i))) in
-    let remaining = to_pos - from_pos in
-    if remaining = 0 then SeqProperties.lemma_contains_empty #(entry r i)
-    else
-      let l0 = minNat remaining blockl in
-      let l_32 = UInt32.uint_to_t l0 in
-      let plain_hd = Crypto.Plain.slice plain from_pos (from_pos + l0) in
-      let cipher_hd = Seq.slice cipher from_pos (from_pos + l0) in
-      let block = PRF.Entry x (PRF.OTP l_32 plain_hd cipher_hd) in 
-      let blocks = counterblocks i r (PRF.incr i x) l (from_pos + l0) to_pos plain cipher in
-      lemma_counterblocks_iv i r (PRF.incr i x) l (from_pos + l0) to_pos plain cipher;
-      SeqProperties.lemma_contains_singleton block;
-      FStar.Classical.forall_intro (SeqProperties.append_contains_equiv (Seq.create 1 block) blocks)
+(* let rec lemma_counterblocks_iv *)
+(*   (i:id{safeId i}) *)
+(*   (r:eternal_region) *)
+(*   (x:PRF.domain i{PRF.ctr_0 i <^ PRF.(x.ctr)}) *)
+(*   (l:nat) *)
+(*   (from_pos:nat) *)
+(*   (to_pos:nat{from_pos <= to_pos /\ to_pos <= l /\ safelen i (to_pos - from_pos) PRF.(x.ctr)}) *)
+(*   (plain:Crypto.Plain.plain i l) *)
+(*   (cipher:lbytes l) : Lemma *)
+(*   (requires True) *)
+(*   (ensures (let otp_entries = counterblocks i r x l from_pos to_pos plain cipher in *)
+(*             forall (prf_entry:entry r i). *)
+(*               otp_entries `SeqProperties.contains` prf_entry ==> prf_entry.x.iv = x.iv)) *)
+(*   (decreases (to_pos - from_pos)) *)
+(*   = let blockl = v (Crypto.Symmetric.Cipher.(blocklen (cipherAlg_of_id i))) in *)
+(*     let remaining = to_pos - from_pos in *)
+(*     if remaining = 0 then SeqProperties.lemma_contains_empty #(entry r i) *)
+(*     else *)
+(*       let l0 = minNat remaining blockl in *)
+(*       let l_32 = UInt32.uint_to_t l0 in *)
+(*       let plain_hd = Crypto.Plain.slice plain from_pos (from_pos + l0) in *)
+(*       let cipher_hd = Seq.slice cipher from_pos (from_pos + l0) in *)
+(*       let block = PRF.Entry x (PRF.OTP l_32 plain_hd cipher_hd) in  *)
+(*       let blocks = counterblocks i r (PRF.incr i x) l (from_pos + l0) to_pos plain cipher in *)
+(*       lemma_counterblocks_iv i r (PRF.incr i x) l (from_pos + l0) to_pos plain cipher; *)
+(*       SeqProperties.lemma_contains_singleton block; *)
+(*       FStar.Classical.forall_intro (SeqProperties.append_contains_equiv (Seq.create 1 block) blocks) *)
 
-val frame_refines_one_entry_snoc
-  (#r:region)
-  (#i:id)
-  (prf_table:prf_table r i)
-  (h:mem{safeId i})
-  (mac_entry:entry r i)
-  (aead_entry:aead_entry i) : Lemma
-  (requires (refines_one_entry prf_table aead_entry h /\
-             not (aead_entry.nonce = mac_entry.x.iv)))
-  (ensures  (refines_one_entry (SeqProperties.snoc prf_table mac_entry) aead_entry h))
-#set-options "--z3rlimit 100"
-let frame_refines_one_entry_snoc #r #i prf_table h mac_entry aead_entry =
-  let open FStar.Classical in
-  forall_intro (move_requires (frame_prf_find_snoc_iv #r #i prf_table mac_entry))
+(* val frame_refines_one_entry_snoc *)
+(*   (#r:region) *)
+(*   (#i:id) *)
+(*   (prf_table:prf_table r i) *)
+(*   (h:mem{safeId i}) *)
+(*   (mac_entry:entry r i) *)
+(*   (aead_entry:aead_entry i) : Lemma *)
+(*   (requires (refines_one_entry prf_table aead_entry h /\ *)
+(*              not (aead_entry.nonce = mac_entry.x.iv))) *)
+(*   (ensures  (refines_one_entry (SeqProperties.snoc prf_table mac_entry) aead_entry h)) *)
+(* #set-options "--z3rlimit 100" *)
+(* let frame_refines_one_entry_snoc #r #i prf_table h mac_entry aead_entry = *)
+(*   let open FStar.Classical in *)
+(*   forall_intro (move_requires (frame_prf_find_snoc_iv #r #i prf_table mac_entry)) *)
 
 (* val aead_inv_after_prf_mac *)
 (*   (#i:id) *)
@@ -245,30 +257,4 @@ let frame_refines_one_entry_snoc #r #i prf_table h mac_entry aead_entry =
 (*        frame_refines i aead_st.prf.mac_rgn prf_table_0 aead_entries h0 h1; *)
 (*        assert (refines prf_table_0 aead_entries h1); *)
 (*        admit()) *)
-(*   end *)
-
-(* val inv_after_prf_mac *)
-(*   (#i:id) *)
-(*   (#rw:rw) *)
-(*   (aead_st:aead_state i rw) *)
-(*   (k_0:CMA.akey aead_st.prf.mac_rgn i) *)
-(*   (x:PRF.domain_mac i) *)
-(*   (mac:CMA.state (i,x.iv)) *)
-(*   (h0 h1:mem) : Lemma *)
-(*   (requires inv aead_st h0 /\                              //invariant holds in h0 *)
-(*             (safeId i ==> fresh_nonce x.iv aead_st h0) /\  //the nonce is fresh w.r.t. the AEAD table *)
-(*             prf_mac_ensures i aead_st.prf k_0 x h0 mac h1) //prf_mac_ensures holds from h0 to h1 *)
-
-(*   (ensures inv aead_st h1 /\                                       //invariant holds in h1 *)
-(*            (safeId i ==>  //TODO: should this be authId i??       *)
-(*              (let prf_table = HS.sel h1 (itable i aead_st.prf) in *)
-(* 	      unused_mac_exists aead_st.prf x h1 /\                //unused mac exists in the prf table *)
-(*               none_above (PRF.incr i x) prf_table)))              //no otp entries exist in the prf table for this nonce *)
-(* #reset-options "--z3rlimit 100 --initial_fuel 0 --max_fuel 0 --initial_ifuel 0 --max_ifuel 0" *)
-(* let inv_after_prf_mac #i #rw aead_st k_0 x mac h0 h1 = *)
-(*   if safeId i *)
-(*   then begin *)
-(*     unused_mac_exists_after_prf_mac aead_st k_0 x mac h0 h1;  //establish unused_mac_exists *)
-(*     none_above_otp_after_prf_mac aead_st k_0 x mac h0 h1;     //establish none_above *)
-(*     () *)
 (*   end *)
